{
 "cells": [
  {
   "cell_type": "markdown",
   "metadata": {
    "id": "4fDEWUHW8MXB"
   },
   "source": [
    "# 7.3 Frechet Derivatives\n",
    "\n",
    "\n"
   ]
  },
  {
   "cell_type": "markdown",
   "metadata": {
    "id": "OfMln32bnDJE"
   },
   "source": [
    "If $T$ is Frechet differentiable, then $\\delta T(x; h) = A_x h$, where $A_x$ is a bounded linear operator from $X$ to $Y$. The Frechet derivative $T': D \\subseteq X \\to B(X, Y)$ of $T$ is defined as the mapping that maps the point $x$ to the bounded operator $A_x$. \n",
    "\n",
    "We say that the Frechet derivative of $T$ is continuous at $x_0$ if the mapping $T'$ is continuous at $x_0$; this is different from say $T'(x_0)$ is continuous - which is always true. If the derivative of $T$ is continuous on some open sphere $S$, we say that $T$ is continuously Frechet differentiable on $S$.\n",
    "\n",
    "> Note: We want $S$ to be open because the definition of continuous function requires an open ball of radius $\\delta$ around the querry point $x_0$.\n",
    "\n",
    "If $f$ is a functional, then $f'(x) \\in X^*$ is called the gradient (which is denoted as $\\nabla f(x)$).\n",
    "\n",
    "Much of the theory of ordinary derivatives can be generalized to Frechet\n",
    "derivatives. For instance, the implicit function theorem and Taylor series\n",
    "have very satisfactory extensions. The interested reader should consult the references cited at the end of the chapter."
   ]
  },
  {
   "cell_type": "markdown",
   "metadata": {
    "id": "jQhMv9w9qGLf"
   },
   "source": [
    "**Claim.** If $T_1$ and $T_2$ are Frechet differentiable at $x\\in D$, then $\\alpha_1 T_1 + \\alpha_2 T_2$ is Frechet differentiable at $x$ and $(\\alpha_1 T_1 + \\alpha_2 T_2)'(x) = \\alpha_1 T_1'(x) + \\alpha_2 T_2'(x).$ "
   ]
  },
  {
   "cell_type": "markdown",
   "metadata": {
    "id": "Ag8ED7Kg7RQu"
   },
   "source": [
    "**Proof.** To show that that $\\alpha_1 T_1 + \\alpha_2 T_2$ is Frechet differentiable, let $x \\in D, h \\in X$ be given. It is true that $\\delta (\\alpha_1 T_1 + \\alpha_2 T_2)(x; h)$ exists, since\n",
    "\\begin{align}\n",
    "\\delta (\\alpha_1 T_1 + \\alpha_2 T_2)(x; h) & = \\lim_{\\alpha \\to 0} \\frac{1}{\\alpha}[(\\alpha_1 T_1 + \\alpha_2 T_2)(x + h) - (\\alpha_1 T_1 + \\alpha_2 T_2)(x)]\\\\\n",
    "& = \\lim_{\\alpha \\to 0} \\frac{1}{\\alpha}[\\alpha_1 T_1(x + h) - \\alpha_1 T_1(x)] + \\lim_{\\alpha \\to 0} \\frac{1}{\\alpha}[\\alpha_2 T_2(x + h) - \\alpha_2 T_2(x)]\\\\\n",
    "& = \\alpha_1 \\delta T_1(x; h) + \\alpha_2 \\delta T_2(x; h).\n",
    "\\end{align}\n",
    "Hence, $\\alpha_1 T_1 + \\alpha_2 T_2$ is Gateux differentiable. Moreover, $\\delta T_1(x; h)$ and $\\delta T_2(x; h)$ are linear and bounded in $h$, meaning that $\\delta (\\alpha_1 T_1 + \\alpha_2 T_2)(x; h)$ is also linear and bounded in $h$. Finally, if we define $T: = \\alpha_1 T_1 + \\alpha_2 T_2$, then \n",
    "\\begin{align}\n",
    "\\lim_{\\lVert h \\rVert \\to 0} & \\frac{\\lVert T(x + h) - T(x) - \\delta T(x; h) \\rVert_Y}{\\lVert h \\rVert_X} \\\\ &\\leq \\lim_{\\lVert h \\rVert \\to 0} \\lvert \\alpha_1 \\rvert \\frac{\\lVert T_1(x + h) - T_1(x) - \\delta T_1(x; h) \\rVert_Y}{\\lVert h \\rVert_X} + \\lim_{\\lVert h \\rVert \\to 0} \\lvert \\alpha_2 \\rvert \\frac{\\lVert T_2(x + h) - T_2(x) - \\delta T_2(x; h) \\rVert_Y}{\\lVert h \\rVert_X},\n",
    "\\end{align}\n",
    "by the triangle inequality. The RHS converges to 0, since $T_1$ and $T_2$ are Frechet differentiable. We also have\n",
    "$\n",
    "\\delta (\\alpha_1 T_1 + \\alpha_2 T_2)(x; h) = \\alpha_1 \\delta T_1(x; h) + \\alpha_2 \\delta T_2(x; h),$ meaning that\n",
    "$$\n",
    "(\\alpha_1 T_1 + \\alpha_2 T_2)'(x) h = \\alpha_1 T_1'(x)h + \\alpha_2 T_2'(x)h.\n",
    "$$\n"
   ]
  },
  {
   "cell_type": "markdown",
   "metadata": {
    "id": "HRAwNmUolrnk"
   },
   "source": [
    "**Proposition 1.** Let $S$ be a transformation mapping an open set $D \\subseteq X$ into an open set $E \\subseteq Y$ and let $P$ be a transformation mapping $E$ into a normed space $Z$. Put $T = PS$ and suppose $S$ is Frechet differentiable at $x \\in D$ and $P$ is Frechet differentiable at $y = S(x) \\in E$. Then $T$ is Frechet differentiable at $x$ and $T'(x) = P'(y) S'(x)$. "
   ]
  },
  {
   "cell_type": "markdown",
   "metadata": {
    "id": "ikiKJq1glrh0"
   },
   "source": [
    "**Proof.**\n",
    "> **Definition**: \n",
    "<br>Little $o$ notation: if $f(x) \\in o(g(x))$ as $x \\to a$, then\n",
    "$$\n",
    "\\lim_{x \\to a} \\frac {f(x)} {g(x)} = 0.\n",
    "$$\n",
    "<br>Big $O$ notation: if $f(x) \\in O(g(x))$  as $x \\to a$, then\n",
    "$$\n",
    "\\lim_{x \\to a}  \\frac {f(x)} {g(x)} < \\infty.\n",
    "$$\n",
    "For both definition, $a$ is not specified, then it is equal to 0.\n",
    "\n",
    "For $h \\in X, x+h \\in D$, we have\n",
    "$$\n",
    "T(x+h)-T(x) = P[S(x+h)]-P[S(x)] = P(y+g)-P(y)\n",
    "$$\n",
    "where $g=S(x+h)-S(x)$. Thus $\\lVert T(x+h)-T(x)-P'(y)g \\rVert = o(\\lVert g \\rVert)$ and $\\lVert g - S'(x)h \\rVert = o(\\lVert h \\rVert)$. We therefore have\n",
    "$$\n",
    "\\lim_{\\lVert h \\rVert \\to 0}\\frac{\\lVert g - S'(x)h \\rVert}{\\lVert h \\rVert} = 0\n",
    "\\Leftrightarrow\n",
    "\\lim_{\\lVert h \\rVert \\to 0}\\frac{g - S'(x)h }{\\lVert h \\rVert} = 0.\n",
    "$$\n",
    "Thus, by continuity and linearity of $P'(y)$, we have\n",
    "$$\n",
    "P'(y) \\lim_{\\lVert h \\rVert \\to 0}\\frac{ g - S'(x)h}{\\lVert h \\rVert} = 0 \\Leftrightarrow\n",
    "\\lim_{\\lVert h \\rVert \\to 0}\\frac{ P'(y) g - P'(y) S'(x)h }{\\lVert h \\rVert} = 0,\n",
    "$$\n",
    "One has $\\lVert g \\rVert = O(\\lVert h \\rVert)$ as $\\lVert h \\rVert \\to 0$ because, by the Frechet diferentiability of $S$ and the fact that since $S'(x)$ is bounded, we have\n",
    "$$\n",
    "\\lim_{\\lVert h \\rVert \\to 0}\\frac{\\lVert g  \\rVert}{\\lVert h \\rVert} = \\lim_{\\lVert h \\rVert \\to 0}\\frac{\\lVert S'(x)h \\rVert}{\\lVert h \\rVert} \\leq \\lim_{\\lVert h \\rVert \\to 0}\\frac{\\lVert S'(x) \\rVert \\lVert h \\rVert}{\\lVert h \\rVert} = \\lVert S'(x) \\rVert < \\infty.\n",
    "$$\n",
    "Then:\n",
    "\\begin{align}\n",
    "&\\lim_{\\lVert h \\rVert \\to 0} \\frac {\\lVert T(x+h)-T(x)-P'(y)S'(x)h \\rVert} {\\lVert h \\rVert} \\\\\n",
    "&\\leq \\lim_{\\lVert h \\rVert \\to 0} \\frac {\\lVert T(x+h)-T(x)-P'(y)g \\rVert} {\\lVert h \\rVert} + \\lim_{\\lVert h \\rVert \\to 0} \\frac{\\lVert P'(y)g -P'(y)S'(x)h \\rVert} {\\lVert h \\rVert}\\\\\n",
    "&= \\lim_{\\lVert h \\rVert \\to 0} \\frac {\\lVert T(x+h)-T(x)-P'(y)g \\rVert} {\\lVert h \\rVert} = \\lim_{\\lVert g \\rVert \\to 0} \\frac {\\lVert P(y+g)-P(y)-P'(y)g \\rVert} {\\lVert g \\rVert} \\lim_{\\lVert h \\rVert \\to 0} \\frac{\\lVert g \\rVert}{\\lVert h \\rVert} \\leq 0 \\cdot \\lVert S'(x) \\rVert = 0.\n",
    "\\end{align}\n",
    "Note that in the last line, we can change from limit of $\\lVert h \\rVert \\to 0$ to $\\lVert g \\rVert \\to 0$ because according to Proposition 3 of Section 7.2, $S$ is continuous at $x$, leading to\n",
    "$$\n",
    "\\lim_{\\lVert h \\rVert \\to 0} g = \\lim_{\\lVert h \\rVert \\to 0} S(x+h)-S(x) = S(x + \\lim_{\\lVert h \\rVert \\to 0}h)-S(x) = S(x) - S(x) = 0.\n",
    "$$\n",
    "\n",
    "\n",
    "Since Frechet differential is unique, we have\n",
    "$$\n",
    "T'(x)h = P'(y)S'(x)h.\n",
    "$$\n",
    "\n",
    "\n"
   ]
  },
  {
   "cell_type": "markdown",
   "metadata": {
    "id": "zxuAplygnYkm"
   },
   "source": [
    "> *Note*: It is also beneficial to learn the short hand argument approach through big $o$ and little $O$ notation presented in Luenberger. We know $\\lVert T(x+h)-T(x)-P'(y)g \\rVert = o(\\lVert g \\rVert)$ and $\\lVert P'(y)g - P'(y)S'(x)h \\rVert = o(\\lVert h \\rVert)$, hence\n",
    "\\begin{align}\n",
    "\\lVert T(x+h)-T(x)- P'(y) S'(x)h \\rVert &\\leq \\lVert T(x+h)-T(x)-P'(y)g \\rVert + \\lVert P'(y)g - P'(y)S'(x)h \\rVert \\\\\n",
    "& = o(\\lVert h \\rVert) + o(\\lVert g \\rVert)\\\\\n",
    "\\Leftrightarrow \\frac{\\lVert T(x+h)-T(x)- P'(y) S'(x)h \\rVert}{\\lVert h \\rVert} & \\leq \\frac{o(\\lVert h \\rVert)}{\\lVert h \\rVert} + \\frac{o(\\lVert g \\rVert)}{\\lVert g \\rVert} \\frac{\\lVert g \\rVert}{\\lVert h \\rVert}\\\\\n",
    "\\end{align}\n",
    "One has $\\lVert g \\rVert = O(\\lVert h \\rVert)$ as $\\lVert h \\rVert \\to 0$ because of the Frechet diferentiability of $S$ and the fact that since $S'(x)$ is bounded. This also implies that $\\lVert g \\rVert \\to 0$ as $\\lVert h \\rVert \\to 0$. Therefore, \n",
    "$$\n",
    "\\frac{\\lVert T(x+h)-T(x)- P'(y) S'(x)h \\rVert}{\\lVert h \\rVert} \\leq \\frac{o(\\lVert h \\rVert)}{\\lVert h \\rVert} + \\frac{o(\\lVert g \\rVert)}{\\lVert g \\rVert} \\frac{O(\\lVert h \\rVert)}{\\lVert h \\rVert}.\\\\\n",
    "$$\n",
    "Taking the limit as $\\lVert h \\rVert \\to 0$ on both sides yield the desired result."
   ]
  },
  {
   "cell_type": "markdown",
   "metadata": {
    "id": "7PVhVxLslrfV"
   },
   "source": [
    "**Proposition 2.** Let $T$ be Frechet diferentiable on a open domain $D$. Let $x \\in D$ and suppose that $x + \\alpha h \\in D$ for all $0 \\leq \\alpha \\leq 1$. Then\n",
    "$$\n",
    "\\lVert T(x+h) - T(x) \\rVert \\leq \\lVert h \\rVert \\sup_{0< \\alpha < 1} \\lVert T'(x+\\alpha h) \\rVert.\n",
    "$$"
   ]
  },
  {
   "cell_type": "markdown",
   "metadata": {
    "id": "ML2g0CW2lrRK"
   },
   "source": [
    "**Proof.** Let $x$ and $h$ be fixed and let $y^*$ be a nonzero element of the dual space $Y^*$ aligned with the element $T(x +h) - T(x)$. Let us remind ourselves that a vector $s^* \\in S^*$ is said to be aligned with a vector $s \\in S$ if $s^*(s) = \\lVert s^* \\rVert \\lVert s \\rVert$.\n",
    "\n",
    "The function $\\varphi(\\alpha) = y^*[T(x+\\alpha h)]$ is defined on the interval $[0, 1]$ and by the chain rule, has derivative\n",
    "$$\n",
    "\\varphi'(\\alpha) = y^*[T'(x + \\alpha h)h].\n",
    "$$\n",
    "> *Note*: This is true since $y^*$ is linear, meaning that $\\delta y^*(y, k) = y^* (k)$ - or $(y^{*})' = y^*$ (by a note from Section 7.2). We can rewrite $T(x + \\alpha h)= T U(\\alpha)$, where $U(\\alpha) = x + \\alpha h$. We can show that $\\delta U(\\alpha; \\beta)$ is linear and continuous and Frechet differentiable. Therefore, $$\\delta U(\\alpha; \\beta) = \\lim_{\\gamma \\to 0} \\frac{1}{\\gamma} [U(\\alpha + \\gamma \\beta) -  U(\\alpha)] = \\beta h = U'(\\alpha) \\beta,$$ meaning that $U'(\\alpha) = h$. \n",
    "\n",
    "\n",
    "By the mean value theorem for functions of a real variable, we have \n",
    "$$\\varphi(1) - \\varphi(0) = \\varphi'(\\alpha_0), \\text{ for some } 0<\\alpha_0 < 1,$$\n",
    "and hence\n",
    "$$\n",
    "\\lvert y^*[T(x + h) - T(x)]\\rvert \\leq \\lVert y^* \\rVert \\sup_{0<\\alpha<1} \\lVert T'(x+\\alpha h) \\rVert \\lVert h \\rVert,\n",
    "$$\n",
    "and since $y^*$ is aligned with $T(x + h) - T(x)$, we have \n",
    "$\n",
    "\\lVert y^* \\rVert  \\lVert T(x + h) - T(x)\\rVert \\leq \\lVert y^* \\rVert \\lVert h \\rVert \\sup_{0<\\alpha<1} \\lVert T'(x+\\alpha h) \\rVert,\n",
    "$\n",
    "which means\n",
    "$$\n",
    "\\lVert T(x + h) - T(x)\\rVert \\leq  \\lVert h \\rVert \\sup_{0<\\alpha<1} \\lVert T'(x+\\alpha h) \\rVert.\n",
    "$$"
   ]
  },
  {
   "cell_type": "markdown",
   "metadata": {
    "id": "F0y0DlXw7iqF"
   },
   "source": [
    "If $T: X \\to Y$ is Frechet differentiable on an open domain $D\\subseteq X$, the derivative $T'$ maps $D$ into $B(X, Y)$ an may itself be Frechet differentiable on a subset $D_t \\subseteq D$. In this case, the Frechet derivative of $T'$ is called the second Frechet derivative of $T$ and is denoted by $T''.$"
   ]
  },
  {
   "cell_type": "markdown",
   "metadata": {
    "id": "n63nYY948SML"
   },
   "source": [
    "> *Note*: The second Frechet derivative $T'': D_t \\subset X \\to B(X, B(X, Y))$, where $B(X, B(X, Y))$ is the space of bounded linear mapping between $X$ and the normed linear space $B(X, Y)$."
   ]
  },
  {
   "cell_type": "markdown",
   "metadata": {
    "id": "yhDc9xgClraG"
   },
   "source": [
    "**Example 1.** Let $f$ be a functional on $X = E^n$ having continuous partial derivatives up to second order. Then $f''(x_0)$ is an operator from $E^n$ to $E^n$ having matrix form\n",
    "$$\n",
    "f''(x_0) = \\left[\\frac{\\partial^2 f(x)}{\\partial x_i \\partial x_j}\\right]_{x = x_0},\n",
    "$$\n",
    "where $x_i$ is the $i$-th component of $x$."
   ]
  },
  {
   "cell_type": "markdown",
   "metadata": {
    "id": "hnQhx3IxlrGK"
   },
   "source": []
  },
  {
   "cell_type": "markdown",
   "metadata": {
    "id": "u4vqDRPVlqrR"
   },
   "source": [
    "**Proposition 3.** Let $T$ be twice Frechet differentiable on an open domain $D$. Let $x\\in D$ and suppose that $x + \\alpha h \\in D$ for all $0\\leq \\alpha \\leq 1$. Then\n",
    "$$\n",
    "\\lVert T(x+h) - T(x) - T'(x)h \\rVert \\leq \\frac{1}{2} \\lVert h \\rVert \\sup_{0< \\alpha < 1} \\lVert T''(x+\\alpha h) \\rVert.\n",
    "$$"
   ]
  }
 ],
 "metadata": {
  "colab": {
   "collapsed_sections": [],
   "name": "7.3 - Frechet Derivatives.ipynb",
   "provenance": []
  },
  "kernelspec": {
   "display_name": "Python 3 (ipykernel)",
   "language": "python",
   "name": "python3"
  },
  "language_info": {
   "codemirror_mode": {
    "name": "ipython",
    "version": 3
   },
   "file_extension": ".py",
   "mimetype": "text/x-python",
   "name": "python",
   "nbconvert_exporter": "python",
   "pygments_lexer": "ipython3",
   "version": "3.7.12"
  }
 },
 "nbformat": 4,
 "nbformat_minor": 1
}
